working on anti

LeanYjs/AntiSymmetry2.lean
@@ -100,11 +100,102 @@ lemma yjs_lt_origin_lt_anti_symm {A} {P : ClosedPredicate A} :
   | lt_first_last =>
     cases hltyx
 
+structure Conflicts {A} (P : ClosedPredicate A) (x y : YjsItem A) where
+  x_origin_y : YjsLt' P x.origin y
+  y_origin_x : YjsLt' P y.origin x
+  x_y_right : YjsLt' P x y.rightOrigin
+  y_x_right : YjsLt' P y x.rightOrigin
+
+lemma conflict_lt_conflicts {A} {P : ClosedPredicate A} :
+  ItemSetInvariant P ->
+  ∀ (x y : YjsPtr A) h, ConflictLt P h x y ->
+    ∃ (x' y' : YjsItem A),
+      x = x' ∧ y = y' ∧ Conflicts P x' y' := by
+  intros inv x y h hltxy
+  cases hltxy with
+  | ltOriginDiff h1 h2 h3 h4 l1 l2 l3 l4 id1 id2 c1 c2 hlt1 hlt2 hlt3 hlt4 =>
+    exists (YjsItem.item l1 l3 id1 c1), (YjsItem.item l2 l4 id2 c2)
+    constructor; simp
+    constructor; simp
+    constructor <;> (unfold YjsLt'; simp [YjsItem.origin, YjsItem.rightOrigin])
+    . constructor; assumption
+    . constructor
+      apply yjs_lt_p_trans inv _ l1 _ _ _ hlt1
+      apply YjsLt.ltOriginOrder
+      apply yjs_lt_p2 hlt1
+      apply yjs_lt_p1 hlt2
+      apply OriginLt.lt_left
+    . constructor; assumption
+    . constructor; assumption
+  | ltOriginSame h1 h2 l r1 r2 id1 id2 c1 c2 hlt1 hlt2 hid =>
+    exists (YjsItem.item l r1 id1 c1), (YjsItem.item l r2 id2 c2)
+    have hpl : P.val l := by
+      obtain ⟨ P, hP ⟩ := P
+      apply hP.closedLeft
+      apply yjs_lt_p1 hlt1
+    have hpr1 : P.val r1 := by
+      obtain ⟨ P, hP ⟩ := P
+      apply hP.closedRight
+      apply yjs_lt_p1 hlt1
+    have hpr2 : P.val r2 := by
+      obtain ⟨ P, hP ⟩ := P
+      apply hP.closedRight
+      apply yjs_lt_p1 hlt2
+    constructor; simp
+    constructor; simp
+    constructor <;> (unfold YjsLt'; simp [YjsItem.origin, YjsItem.rightOrigin])
+    . constructor
+      apply YjsLt.ltOriginOrder <;> try assumption
+      apply yjs_lt_p1 hlt2
+      apply OriginLt.lt_left
+    . constructor
+      apply YjsLt.ltOriginOrder <;> try assumption
+      apply yjs_lt_p1 hlt1
+      apply OriginLt.lt_left
+    . constructor; assumption
+    . constructor; assumption
+
 lemma yjs_lt_conflict_lt_anti_symm {A} {P : ClosedPredicate A} :
   ItemSetInvariant P ->
-  ∀ (x y : YjsPtr A) h1 h2, ConflictLt P h1 x y -> ConflictLt P h2 y x -> False := by
+  ∀ (x y : YjsPtr A) h1 h2, ConflictLt P h1 x y -> ConflictLt P h2 y x ->
+    ∃ (x' y' : YjsPtr A) (h1' h2' : ℕ),
+      YjsLt P h1' x' y' ∧ YjsLt P h2' y' x' ∧ x'.size + y'.size < x.size + y.size := by
   intros inv x y h1 h2 hltxy hltyx
-  sorry
+  cases hltxy with
+  | ltOriginDiff h1' h2' h3' h4' l1 l2 l3 l4 id1 id2 c1 c2 hlt1 hlt2 hlt3 hlt4 =>
+    cases hltyx with
+    | ltOriginDiff h1'' h2'' h3'' h4'' l1' l2' l3' l4' id1' id2' c1' c2' hlt1' hlt2' hlt3' hlt4' =>
+      exists l1, l2
+      constructor
+      constructor
+      constructor; assumption
+      constructor; assumption
+      simp [YjsPtr.size]
+      simp [YjsItem.size]
+      omega
+    | ltOriginSame h1'' h2'' l r1 r2 id1' id2' c1' c2' hlt1' hlt2' hid =>
+      exists l1, l1
+      constructor
+      constructor
+      constructor; assumption
+      constructor; assumption
+      simp [YjsPtr.size]
+      simp [YjsItem.size]
+      omega
+  | ltOriginSame h1' h2' l r1 r2 id1 id2 c1 c2 hlt1 hlt2 hid =>
+    cases hltyx with
+    | ltOriginDiff h1'' h2'' h3'' h4'' l1' l2' l3' l4' id1' id2' c1' c2' hlt1' hlt2' hlt3' hlt4' =>
+      exists l, l
+      constructor
+      constructor
+      constructor; assumption
+      constructor; assumption
+      simp [YjsPtr.size]
+      simp [YjsItem.size]
+      omega
+    | ltOriginSame h1'' h2'' l r1 r2 id1' id2' c1' c2' hlt1' hlt2' hid =>
+      unfold ActorId at *
+      omega
 
 theorem yjs_lt_anti_symm {A} {P : ClosedPredicate A} :
   ItemSetInvariant P ->
@@ -122,7 +213,7 @@ theorem yjs_lt_anti_symm {A} {P : ClosedPredicate A} :
   | ltTrans h1' h2' x t y hltxy hltyz =>
     have hltxy' : YjsLt P (max h1' (h2' + 1) + 1) x t := by
       apply yjs_lt_p_trans _ _ y _ <;> try assumption
-      
+
   | ltConflict h1' x' y' hltx'y' =>
     cases hltyx with
     | ltConflict h2' x'' y'' hlty'x''y'' =>
